src/Framework/Layer/Layer.v
@@ -1,2 +1,2 @@
-Require Export  Layer.Operation Layer.Language
+Require Export  Layer.Core Layer.Language
         Layer.HorizontalComposition Layer.Automation.
